Pull-out: factorize.lean

src/common.lean
@@ -1,8 +1,4 @@
-import data.list data.list.sort data.bool
-import tactic.norm_num tactic.omega
-
-attribute [simp, reducible] nat.factors
-attribute [simp, reducible] ite
+import tactic.omega
 
 notation `ℙ` := nat.primes
 
@@ -57,60 +53,3 @@ def seg (a b: ℕ) := (list.range (b-a)).map(λ x, x+a)
 def find {α: Type} (p: α -> Prop) [decidable_pred p] [inhabited α] : list α -> α
 | [] := arbitrary α
 | (h::t) := cond (p h) h (find t)
-
-@[simp, reducible]
-def list.uniq {α: Type*} [decidable_eq α]: list α -> list α
-| [] := []
-| [a] := [a]
-| (a::b::t) := cond (a = b) (list.uniq (b::t)) (a::(list.uniq (b::t)))
-
--- factorize n = the list of pairs [(p1, e1), ..., (pm, em)], where Π pi^ei = n
-@[simp, reducible]
-def factorize (n: ℕ) : list (ℕ × ℕ) := 
-  let l := tree_sort.sort (λ a b, to_bool (a < b)) (nat.factors n) in
-  let (c: list ℕ) := list.map (λ x, list.count x l) l in
-  let l' := tree_sort.sort (λ a b, to_bool (a < b)) (list.zip l c) in
-  l'.uniq
-
-#eval factorize (2*2*3*5*5)
-
-example: factorize (2*2*3*5*5) = [(2, 2), (3, 1), (5, 2)] := begin
-norm_num,
-reflexivity,
-end
-
-@[simp, reducible]
-def list.subl {α: Type*} [has_lt α] [decidable_eq α] [decidable_rel ((<) : α → α → Prop)]: list α -> list (list α)
-| [] := [[]]
-| (h::t) := 
-  let sort := tree_sort.sort (λ (x y: list α), x.length < y.length) in
-  let ss := sort ((list.subl t) ++ (list.subl t).map(list.cons h)) in
-  (tree_sort.sort (λ (x y: list α), to_bool ((x.length, x) < (y.length, y))) ss).uniq
-
-#eval (nat.factors (2*2*3*5*5)).subl
-@[simp, reducible]
-def divisors_factorized (n: ℕ) :=
-  (tree_sort.sort (λ s t, (list.length s) < (list.length t)) (nat.factors n).subl)
-
-#eval divisors_factorized (2*2*3*5*5)
-example: divisors_factorized (2*2*3*5*5) = [
-  [], [5], [3], [2], [5, 5], [3, 5], [2, 5], [2, 3], 
-  [2, 2], [3, 5, 5], [2, 5, 5], [2, 3, 5], [2, 2, 5], [2, 2, 3], [2, 3, 5, 5], 
-  [2, 2, 5, 5], [2, 2, 3, 5], [2, 2, 3, 5, 5]
-] := begin
-norm_num,
-reflexivity,
-end 
-
-#eval divisors_factorized (2*2*3*5*5)
-
-@[simp, reducible]
-def divisors (n: ℕ) := 
-  tree_sort.sort (λ x y, to_bool (x < y)) ((divisors_factorized n).map list.prod)
-
-#eval divisors (2*2*3*5*5)
-example: divisors (2*2*3*5*5) = [1, 2, 3, 4, 5, 6, 10, 12, 15, 20, 25, 30, 50, 60, 75, 100, 150, 300] := begin
-norm_num,
-reflexivity,
-end
-
